more binary search

examples/binary_search.v
@@ -5,29 +5,101 @@ Require Import isla.adequacy.
 Require Import isla.examples.sys_regs.
 From isla.instructions.binary_search Require Import instrs.
 
+Definition args_registers : list string :=
+  ["R0"; "R1"; "R2"; "R3"; "R4"; "R5"; "R6"; "R7"].
+Definition tmp_registers : list string :=
+  ["R9"; "R10"; "R11"; "R12"; "R13"; "R14"; "R15"; "R16"; "R17"].
 
-(*
-The code can be generated with
-PATH=$PWD/bin:$PATH dune exec -- isla-coq examples/binary_search.dump -d -o instructions/binary_search  -n "a{addr}" --coqdir=isla.instructions.binary_search
 
-*)
+Definition c_call `{!islaG Σ} `{!threadG} (args : list (bv 64)) (P : iProp Σ) (Q : list (bv 64) → iProp Σ) : iProp Σ :=
+  ∃ (ret : bv 64),
+  ∃ (sp r8 r19 r20 r21 r22 r23 r24 r25 r26 r27 r28 r29 : bv 64),
+  reg_col sys_regs ∗
+  reg_col CNVZ_regs ∗
+  reg_col ((λ r, (RegColDirect r, None)) <$> tmp_registers) ∗
+  ([∗ list] r;a∈args_registers;args, r ↦ᵣ Val_Bits (a : bv 64)) ∗
+  "R8" ↦ᵣ Val_Bits r8 ∗
+  "R19" ↦ᵣ Val_Bits r19 ∗
+  "R20" ↦ᵣ Val_Bits r20 ∗
+  "R21" ↦ᵣ Val_Bits r21 ∗
+  "R22" ↦ᵣ Val_Bits r22 ∗
+  "R23" ↦ᵣ Val_Bits r23 ∗
+  "R24" ↦ᵣ Val_Bits r24 ∗
+  "R25" ↦ᵣ Val_Bits r25 ∗
+  "R26" ↦ᵣ Val_Bits r26 ∗
+  "R27" ↦ᵣ Val_Bits r27 ∗
+  "R28" ↦ᵣ Val_Bits r28 ∗
+  "R29" ↦ᵣ Val_Bits r29 ∗
+  "R30" ↦ᵣ Val_Bits ret ∗
+  "SP_EL2" ↦ᵣ Val_Bits sp ∗
+  P ∗
+  instr_pre (bv_unsigned ret) (
+    ∃ (r0 r1 r2 r3 r4 r5 r6 r7 r8 : bv 64),
+      reg_col sys_regs ∗
+      reg_col CNVZ_regs ∗
+      "R0" ↦ᵣ Val_Bits r0 ∗
+      "R1" ↦ᵣ Val_Bits r1 ∗
+      "R2" ↦ᵣ Val_Bits r2 ∗
+      "R3" ↦ᵣ Val_Bits r3 ∗
+      "R4" ↦ᵣ Val_Bits r4 ∗
+      "R5" ↦ᵣ Val_Bits r5 ∗
+      "R6" ↦ᵣ Val_Bits r6 ∗
+      "R7" ↦ᵣ Val_Bits r7 ∗
+      "R8" ↦ᵣ Val_Bits r8 ∗
+      reg_col ((λ r, (RegColDirect r, None)) <$> tmp_registers) ∗
+      "R19" ↦ᵣ Val_Bits r19 ∗
+      "R20" ↦ᵣ Val_Bits r20 ∗
+      "R21" ↦ᵣ Val_Bits r21 ∗
+      "R22" ↦ᵣ Val_Bits r22 ∗
+      "R23" ↦ᵣ Val_Bits r23 ∗
+      "R24" ↦ᵣ Val_Bits r24 ∗
+      "R25" ↦ᵣ Val_Bits r25 ∗
+      "R26" ↦ᵣ Val_Bits r26 ∗
+      "R27" ↦ᵣ Val_Bits r27 ∗
+      "R28" ↦ᵣ Val_Bits r28 ∗
+      "R29" ↦ᵣ Val_Bits r29 ∗
+      "R30" ↦ᵣ Val_Bits ret ∗
+      "SP_EL2" ↦ᵣ Val_Bits sp ∗
+      Q [r0; r1; r2; r3; r4; r5; r6; r7; r8] ∗
+      True
+  ).
+
+Arguments c_call _ _ _ /.
+
+Definition comp_spec `{!islaG Σ} `{!threadG} : iProp Σ :=
+  ∃ r0 r1 r2 r3 r4 r5 r6 r7,
+  c_call [r0; r1; r2; r3; r4; r5; r6; r7] True (λ rets, True).
+
 
 Definition binary_search_loop_spec `{!islaG Σ} `{!threadG} : iProp Σ :=
-  ∃ (tmp src dst i n : bv 64) (srcdata dstdata : list byte) (pstaten pstatez pstatec pstatev : bv 1),
+  ∃ (x l r comp xs tmp2 tmp5 : bv 64) (data : list (bv 64)),
   reg_col sys_regs ∗
-  "PSTATE" # "N" ↦ᵣ Val_Bits pstaten ∗ "PSTATE" # "Z" ↦ᵣ Val_Bits pstatez ∗
-  "PSTATE" # "C" ↦ᵣ Val_Bits pstatec ∗ "PSTATE" # "V" ↦ᵣ Val_Bits pstatev ∗
-  "R0" ↦ᵣ Val_Bits dst ∗ "R1" ↦ᵣ Val_Bits src ∗ "R2" ↦ᵣ Val_Bits n ∗
-  "R3" ↦ᵣ Val_Bits i ∗ "R4" ↦ᵣ Val_Bits tmp ∗
-  src ↦ₘ∗ srcdata ∗ dst ↦ₘ∗ dstdata ∗
+  reg_col CNVZ_regs ∗
+  reg_col ((λ r, (RegColDirect r, None)) <$> ["R0"; "R1"; "R2"; "R3"; "R4"; "R5"; "R6"; "R7"; "R8"; "R9"; "R10"; "R11"; "R12"; "R13"; "R14"; "R15"; "R16"; "R17" ]) ∗
+  "R19" ↦ᵣ Val_Bits x ∗
+  "R20" ↦ᵣ Val_Bits r ∗
+  "R21" ↦ᵣ Val_Bits xs ∗
+  "R22" ↦ᵣ Val_Bits comp ∗
+  "R23" ↦ᵣ Val_Bits l ∗
+  "R24" ↦ᵣ Val_Bits tmp2 ∗
+  "R30" ↦ᵣ Val_Bits tmp5 ∗
+  xs ↦ₘ∗ data ∗
+  ⌜bv_unsigned l < bv_unsigned r ≤ length data⌝ ∗
+  ⌜bv_unsigned xs + (length data) * 8 < 2 ^ 52⌝ ∗
+  □ instr_pre (bv_unsigned comp) comp_spec ∗
   instr_pre 0x0000000010300054 (
-    ∃ (tmp n : bv 64) (pstaten pstatez pstatec pstatev : bv 1),
+    ∃ (tmp2 tmp5 : bv 64),
       reg_col sys_regs ∗
-      "PSTATE" # "N" ↦ᵣ Val_Bits pstaten ∗ "PSTATE" # "Z" ↦ᵣ Val_Bits pstatez ∗
-      "PSTATE" # "C" ↦ᵣ Val_Bits pstatec ∗ "PSTATE" # "V" ↦ᵣ Val_Bits pstatev ∗
-      "R0" ↦ᵣ Val_Bits dst ∗ "R1" ↦ᵣ Val_Bits src ∗ "R2" ↦ᵣ Val_Bits n ∗
-      "R4" ↦ᵣ Val_Bits tmp ∗ "R3" ↦ᵣ Val_Bits n ∗
-      src ↦ₘ∗ srcdata ∗ dst ↦ₘ∗ srcdata ∗
+      reg_col CNVZ_regs ∗
+      reg_col ((λ r, (RegColDirect r, None)) <$> ["R0"; "R1"; "R2"; "R3"; "R4"; "R5"; "R6"; "R7"; "R8"; "R9"; "R10"; "R11"; "R12"; "R13"; "R14"; "R15"; "R16"; "R17" ]) ∗
+      "R19" ↦ᵣ Val_Bits x ∗
+      "R20" ↦ᵣ Val_Bits r ∗
+      "R21" ↦ᵣ Val_Bits xs ∗
+      "R22" ↦ᵣ Val_Bits comp ∗
+      "R23" ↦ᵣ Val_Bits l ∗
+      "R24" ↦ᵣ Val_Bits tmp2 ∗
+      "R30" ↦ᵣ Val_Bits tmp5 ∗
+      xs ↦ₘ∗ data ∗
       True
   )
 .
@@ -50,6 +122,11 @@ Lemma binary_search_loop `{!islaG Σ} `{!threadG} :
 Proof.
   iStartProof.
   Time repeat liAStep; liShow.
+  liInst Hevar (Z.to_nat (bv_unsigned l + (bv_unsigned r - bv_unsigned l) `div` 2)).
+  Time repeat liAStep; liShow.
+  iEval (rewrite /comp_spec /=).
+  Time repeat liAStep; liShow.
+
 Abort.
 
 Lemma binary_search `{!islaG Σ} `{!threadG} :
@@ -75,18 +152,16 @@ Lemma binary_search `{!islaG Σ} `{!threadG} :
   instr 0x0000000010300070 (Some a70) -∗
   □ instr_pre 0x000000001030002c binary_search_loop_spec -∗
   instr_body 0x0000000010300000 (
-    ∃ (tmp1 tmp2 src dst n ret : bv 64) (srcdata dstdata : list byte) (pstaten pstatez pstatec pstatev : bv 1),
+    ∃ (tmp1 tmp2 src dst n ret : bv 64) (srcdata dstdata : list byte),
     reg_col sys_regs ∗
-    "PSTATE" # "N" ↦ᵣ Val_Bits pstaten ∗ "PSTATE" # "Z" ↦ᵣ Val_Bits pstatez ∗
-    "PSTATE" # "C" ↦ᵣ Val_Bits pstatec ∗ "PSTATE" # "V" ↦ᵣ Val_Bits pstatev ∗
+    reg_col CNVZ_regs ∗
     "R0" ↦ᵣ Val_Bits dst ∗ "R1" ↦ᵣ Val_Bits src ∗ "R2" ↦ᵣ Val_Bits n ∗
     "R3" ↦ᵣ Val_Bits tmp2 ∗ "R4" ↦ᵣ Val_Bits tmp1 ∗
     "R30" ↦ᵣ Val_Bits ret ∗
     instr_pre (bv_unsigned ret) (
-    ∃ (tmp1 tmp2 n : bv 64) (pstaten pstatez pstatec pstatev : bv 1),
+    ∃ (tmp1 tmp2 n : bv 64),
       reg_col sys_regs ∗
-      "PSTATE" # "N" ↦ᵣ Val_Bits pstaten ∗ "PSTATE" # "Z" ↦ᵣ Val_Bits pstatez ∗
-      "PSTATE" # "C" ↦ᵣ Val_Bits pstatec ∗ "PSTATE" # "V" ↦ᵣ Val_Bits pstatev ∗
+      reg_col CNVZ_regs ∗
       "R0" ↦ᵣ Val_Bits dst ∗ "R1" ↦ᵣ Val_Bits src ∗ "R2" ↦ᵣ Val_Bits n ∗
       "R3" ↦ᵣ Val_Bits tmp2 ∗ "R4" ↦ᵣ Val_Bits tmp1 ∗
       "R30" ↦ᵣ Val_Bits ret ∗
